Add assumptions context.
Have not encoded the rules yet.

theories/lang_oadt/properties.v
@@ -1,12 +1,12 @@
-From oadt Require Import prelude.
+From oadt Require Import lang_oadt.base.
 From oadt Require Import lang_oadt.infrastructure.
 
 (** * Properties *)
 (** Lemmas for various definitions. *)
 
-Module M (atom_sig : AtomSig).
+Module M (sig : OADTSig).
 
-Include infrastructure.M atom_sig.
+Include infrastructure.M sig.
 Import syntax_notations.
 Import semantics_notations.
 Import typing_notations.
@@ -53,20 +53,20 @@ Hint Constructors whnf : whnf.
 
 (** Type equivalence for the weak head normal form fragments. This relation
 always assumes that the two type arguments are already in [whnf]. *)
-Inductive whnf_equiv {Σ : gctx} : expr -> expr -> Prop :=
+Inductive whnf_equiv {Σ : gctx} {Φ : actx} : expr -> expr -> Prop :=
 | WEqUnitT : whnf_equiv <{ 𝟙 }> <{ 𝟙 }>
 | WEqBool l : whnf_equiv <{ 𝔹{l} }> <{ 𝔹{l} }>
 | WEqPi τ1 τ2 τ1' τ2' :
-    Σ ⊢ τ1 ≡ τ1' ->
-    Σ ⊢ τ2 ≡ τ2' ->
+    Σ; Φ ⊢ τ1 ≡ τ1' ->
+    Σ; Φ ⊢ τ2 ≡ τ2' ->
     whnf_equiv <{ Π:τ1, τ2 }> <{ Π:τ1', τ2' }>
 | WEqProd τ1 τ2 τ1' τ2' :
-    Σ ⊢ τ1 ≡ τ1' ->
-    Σ ⊢ τ2 ≡ τ2' ->
+    Σ; Φ ⊢ τ1 ≡ τ1' ->
+    Σ; Φ ⊢ τ2 ≡ τ2' ->
     whnf_equiv <{ τ1 * τ2 }> <{ τ1' * τ2' }>
 | WEqSum l τ1 τ2 τ1' τ2' :
-    Σ ⊢ τ1 ≡ τ1' ->
-    Σ ⊢ τ2 ≡ τ2' ->
+    Σ; Φ ⊢ τ1 ≡ τ1' ->
+    Σ; Φ ⊢ τ2 ≡ τ2' ->
     whnf_equiv <{ τ1 +{l} τ2 }> <{ τ1' +{l} τ2' }>
 | WEqADT X : whnf_equiv <{ gvar X }> <{ gvar X }>
 .
@@ -82,94 +82,96 @@ Qed.
 
 (** ** Properties of type equivalence  *)
 
-Instance expr_equiv_is_equiv Σ : Equivalence (expr_equiv Σ).
+Instance expr_equiv_is_equiv Σ Φ : Equivalence (expr_equiv Σ Φ).
 Proof.
 Admitted.
 
 (** [whnf_equiv] is a faithful fragment of [expr_equiv]. *)
-Lemma expr_equiv_iff_whnf_equiv Σ τ1 τ2 :
+Lemma expr_equiv_iff_whnf_equiv Σ Φ τ1 τ2 :
   whnf Σ τ1 -> whnf Σ τ2 ->
-  Σ ⊢ τ1 ≡ τ2 <->
-  whnf_equiv Σ τ1 τ2.
+  Σ; Φ ⊢ τ1 ≡ τ2 <->
+  whnf_equiv Σ Φ τ1 τ2.
 Proof.
 Admitted.
 
 (* NOTE: Be aware of circular proofs! In case we need [gctx_wf] as a side
 condition, as we need this lemma to prove [gctx_wf] for well-typed global
 context. *)
-Lemma expr_equiv_weakening Σ τ τ' :
-  Σ ⊢ τ ≡ τ' ->
-  forall Σ', Σ ⊆ Σ' ->
-        Σ' ⊢ τ ≡ τ'.
+Lemma expr_equiv_weakening Σ Φ τ τ' :
+  Σ; Φ ⊢ τ ≡ τ' ->
+  forall Σ' Φ',
+    Σ ⊆ Σ' ->
+    Φ ⊆ Φ' ->
+    Σ'; Φ' ⊢ τ ≡ τ'.
 Admitted.
 
 (* Some side conditions may be needed for the next few lemmas. *)
 
-Lemma expr_equiv_step Σ e e' :
+Lemma expr_equiv_step Σ Φ e e' :
   Σ ⊨ e -->! e' ->
-  Σ ⊢ e ≡ e'.
+  Σ; Φ ⊢ e ≡ e'.
 Proof.
 Admitted.
 
-Lemma expr_equiv_subst Σ τ τ' e e' x :
-  Σ ⊢ τ ≡ τ' ->
-  Σ ⊢ e ≡ e' ->
-  Σ ⊢ {x↦e}τ ≡ {x↦e'}τ'.
+Lemma expr_equiv_subst Σ Φ τ τ' e e' x :
+  Σ; Φ ⊢ τ ≡ τ' ->
+  Σ; Φ ⊢ e ≡ e' ->
+  Σ; Φ ⊢ {x↦e}τ ≡ {x↦e'}τ'.
 Proof.
 Admitted.
 
-Lemma expr_equiv_open_atom Σ τ1 τ2 x :
-  Σ ⊢ τ1 ≡ τ2 ->
-  Σ ⊢ τ1^x ≡ τ2^x.
+Lemma expr_equiv_open_atom Σ Φ τ1 τ2 x :
+  Σ; Φ ⊢ τ1 ≡ τ2 ->
+  Σ; Φ ⊢ τ1^x ≡ τ2^x.
 Proof.
 Admitted.
 
 (* We may weaken it so Γ = ∅. But we need to weaken all theorems depending on
 it. *)
-Lemma expr_equiv_obliv_type_preserve_ Σ Γ τ τ' κ κ' :
+Lemma expr_equiv_obliv_type_preserve_ Σ Φ Γ τ τ' κ κ' :
   gctx_wf Σ ->
-  Σ; Γ ⊢ τ :: κ ->
-  Σ; Γ ⊢ τ' :: κ' ->
-  Σ ⊢ τ ≡ τ' ->
+  Σ; Φ; Γ ⊢ τ :: κ ->
+  Σ; Φ; Γ ⊢ τ' :: κ' ->
+  Σ; Φ ⊢ τ ≡ τ' ->
   κ ⊑ <{ *@O }> ->
-  Σ; Γ ⊢ τ' :: *@O.
+  Σ; Φ; Γ ⊢ τ' :: *@O.
 Proof.
 Admitted.
 
-Lemma expr_equiv_obliv_type_preserve Σ Γ τ τ' κ :
+Lemma expr_equiv_obliv_type_preserve Σ Φ Γ τ τ' κ :
   gctx_wf Σ ->
-  Σ; Γ ⊢ τ :: *@O ->
-  Σ ⊢ τ ≡ τ' ->
-  Σ; Γ ⊢ τ' :: κ ->
-  Σ; Γ ⊢ τ' :: *@O.
+  Σ; Φ; Γ ⊢ τ :: *@O ->
+  Σ; Φ ⊢ τ ≡ τ' ->
+  Σ; Φ; Γ ⊢ τ' :: κ ->
+  Σ; Φ; Γ ⊢ τ' :: *@O.
 Proof.
   qauto use: expr_equiv_obliv_type_preserve_ solve: lattice_naive_solver.
 Qed.
 
-Lemma expr_equiv_rename Σ τ τ' x y :
-  Σ ⊢ τ ≡ τ' ->
-  Σ ⊢ {x↦y}τ ≡ {x↦y}τ'.
+Lemma expr_equiv_rename Σ Φ τ τ' x y :
+  Σ; Φ ⊢ τ ≡ τ' ->
+  Σ; Φ ⊢ {x↦y}τ ≡ {x↦y}τ'.
 Proof.
   qauto use: expr_equiv_subst solve: equiv_naive_solver.
 Qed.
 
-Lemma expr_equiv_subst1 Σ τ τ' x s :
-  Σ ⊢ τ ≡ τ' ->
-  Σ ⊢ {x↦s}τ ≡ {x↦s}τ'.
+Lemma expr_equiv_subst1 Σ Φ τ τ' x s :
+  Σ; Φ ⊢ τ ≡ τ' ->
+  Σ; Φ ⊢ {x↦s}τ ≡ {x↦s}τ'.
 Proof.
   qauto use: expr_equiv_subst solve: equiv_naive_solver.
 Qed.
 
-Lemma expr_equiv_subst2 Σ τ x e e' :
-  Σ ⊢ e ≡ e' ->
-  Σ ⊢ {x↦e}τ ≡ {x↦e'}τ.
+Lemma expr_equiv_subst2 Σ Φ τ x e e' :
+  Σ; Φ ⊢ e ≡ e' ->
+  Σ; Φ ⊢ {x↦e}τ ≡ {x↦e'}τ.
 Proof.
   qauto use: expr_equiv_subst solve: equiv_naive_solver.
 Qed.
 
-Lemma expr_equiv_open1 Σ τ1 τ2 e :
-  Σ ⊢ τ1 ≡ τ2 ->
-  Σ ⊢ τ1^e ≡ τ2^e.
+Lemma expr_equiv_open1 Σ Φ τ1 τ2 e :
+  Σ; Φ ⊢ τ1 ≡ τ2 ->
+  Σ; Φ ⊢ τ1^e ≡ τ2^e.
 Proof.
   destruct (exist_fresh (fv τ1 ∪ fv τ2)) as [x ?].
   erewrite (subst_intro τ1 e x) by fast_set_solver!!.
@@ -177,9 +179,9 @@ Proof.
   eauto using expr_equiv_subst1, expr_equiv_open_atom.
 Qed.
 
-Lemma expr_equiv_open2 Σ τ e1 e2 :
-  Σ ⊢ e1 ≡ e2 ->
-  Σ ⊢ τ^e1 ≡ τ^e2.
+Lemma expr_equiv_open2 Σ Φ τ e1 e2 :
+  Σ; Φ ⊢ e1 ≡ e2 ->
+  Σ; Φ ⊢ τ^e1 ≡ τ^e2.
 Proof.
   destruct (exist_fresh (fv τ)) as [x ?].
   erewrite (subst_intro τ e1 x) by eassumption.
@@ -191,7 +193,7 @@ Qed.
 two equivalent types in [whnf] have different head. *)
 Tactic Notation "simpl_whnf_equiv" "by" tactic3(tac) :=
   match goal with
-  | H : _ ⊢ ?τ1 ≡ ?τ2 |- _ =>
+  | H : _; _ ⊢ ?τ1 ≡ ?τ2 |- _ =>
     apply expr_equiv_iff_whnf_equiv in H;
     [ sinvert H
     | solve [tac]
@@ -207,7 +209,7 @@ Tactic Notation "simpl_whnf_equiv" :=
 (** ** Kind inversion  *)
 Tactic Notation "kind_inv_solver" "by" tactic3(tac) :=
   match goal with
-  | |- _; _ ⊢ ?τ :: _ -> _ => remember τ
+  | |- _; _; _ ⊢ ?τ :: _ -> _ => remember τ
   end;
   induction 1; subst; simp_hyps; simplify_eq;
   tac.
@@ -215,171 +217,171 @@ Tactic Notation "kind_inv_solver" "by" tactic3(tac) :=
 Tactic Notation "kind_inv_solver" :=
   kind_inv_solver by (repeat esplit; eauto; lattice_naive_solver).
 
-Lemma kind_inv_pi Σ Γ τ1 τ2 κ :
-  Σ; Γ ⊢ Π:τ1, τ2 :: κ ->
+Lemma kind_inv_pi Σ Φ Γ τ1 τ2 κ :
+  Σ; Φ; Γ ⊢ Π:τ1, τ2 :: κ ->
   κ = <{ *@M }> /\
   exists L κ1 κ2,
-    (∀ x, x ∉ L → Σ; (<[x:=τ1]> Γ) ⊢ τ2^x :: κ2) /\
-    Σ; Γ ⊢ τ1 :: κ1.
+    (∀ x, x ∉ L → Σ; Φ; (<[x:=τ1]> Γ) ⊢ τ2^x :: κ2) /\
+    Σ; Φ; Γ ⊢ τ1 :: κ1.
 Proof.
   kind_inv_solver by sfirstorder use: top_inv.
 Qed.
 
-Lemma kind_inv_bool Σ Γ κ :
-  Σ; Γ ⊢ 𝔹 :: κ -> <{ *@P }> ⊑ κ.
+Lemma kind_inv_bool Σ Φ Γ κ :
+  Σ; Φ; Γ ⊢ 𝔹 :: κ -> <{ *@P }> ⊑ κ.
 Proof.
   kind_inv_solver.
 Qed.
 
-Lemma kind_inv_prod Σ Γ τ1 τ2 κ :
-  Σ; Γ ⊢ τ1 * τ2 :: κ ->
+Lemma kind_inv_prod Σ Φ Γ τ1 τ2 κ :
+  Σ; Φ; Γ ⊢ τ1 * τ2 :: κ ->
   exists κ',
-    Σ; Γ ⊢ τ1 :: κ' /\
-    Σ; Γ ⊢ τ2 :: κ' /\
+    Σ; Φ; Γ ⊢ τ1 :: κ' /\
+    Σ; Φ; Γ ⊢ τ2 :: κ' /\
     <{ κ' }> ⊑ κ.
 Proof.
   kind_inv_solver.
 Qed.
 
-Lemma kind_inv_sum Σ Γ τ1 τ2 κ :
-  Σ; Γ ⊢ τ1 + τ2 :: κ ->
+Lemma kind_inv_sum Σ Φ Γ τ1 τ2 κ :
+  Σ; Φ; Γ ⊢ τ1 + τ2 :: κ ->
   <{ *@P }> ⊑ κ /\
   exists κ',
-    Σ; Γ ⊢ τ1 :: κ' /\
-    Σ; Γ ⊢ τ2 :: κ'.
+    Σ; Φ; Γ ⊢ τ1 :: κ' /\
+    Σ; Φ; Γ ⊢ τ2 :: κ'.
 Proof.
   kind_inv_solver by qauto l: on solve: lattice_naive_solver
                            use: join_ub_r.
 Qed.
 
-Lemma kind_inv_osum Σ Γ τ1 τ2 κ :
-  Σ; Γ ⊢ τ1 ~+ τ2 :: κ ->
+Lemma kind_inv_osum Σ Φ Γ τ1 τ2 κ :
+  Σ; Φ; Γ ⊢ τ1 ~+ τ2 :: κ ->
   <{ *@O }> ⊑ κ /\
-  Σ; Γ ⊢ τ1 :: *@O /\
-  Σ; Γ ⊢ τ2 :: *@O.
+  Σ; Φ; Γ ⊢ τ1 :: *@O /\
+  Σ; Φ; Γ ⊢ τ2 :: *@O.
 Proof.
   kind_inv_solver.
 Qed.
 
-Lemma kind_inv_gvar Σ Γ X κ :
-  Σ; Γ ⊢ gvar X :: κ ->
+Lemma kind_inv_gvar Σ Φ Γ X κ :
+  Σ; Φ; Γ ⊢ gvar X :: κ ->
   <{ *@P }> ⊑ κ /\ exists τ, Σ !! X = Some (DADT τ).
 Proof.
   kind_inv_solver.
 Qed.
 
-Lemma kind_inv_app Σ Γ e1 e2 κ :
-  Σ; Γ ⊢ e1 e2 :: κ ->
+Lemma kind_inv_app Σ Φ Γ e1 e2 κ :
+  Σ; Φ; Γ ⊢ e1 e2 :: κ ->
   <{ *@O }> ⊑ κ /\
   exists X τ e',
     Σ !! X = Some (DOADT τ e') /\
-    Σ; Γ ⊢ e2 : τ /\
+    Σ; Φ; Γ ⊢ e2 : τ /\
     e1 = <{ gvar X }>.
 Proof.
   kind_inv_solver.
 Qed.
 
-Lemma kind_inv_ite Σ Γ l e0 τ1 τ2 κ :
-  Σ; Γ ⊢ if{l} e0 then τ1 else τ2 :: κ ->
+Lemma kind_inv_ite Σ Φ Γ l e0 τ1 τ2 κ :
+  Σ; Φ; Γ ⊢ if{l} e0 then τ1 else τ2 :: κ ->
   <{ *@O }> ⊑ κ /\
   l = ⊥ /\
-  Σ; Γ ⊢ e0 : 𝔹 /\
-  Σ; Γ ⊢ τ1 :: *@O /\
-  Σ; Γ ⊢ τ2 :: *@O.
+  Σ; Φ; Γ ⊢ e0 : 𝔹 /\
+  Σ; Φ; Γ ⊢ τ1 :: *@O /\
+  Σ; Φ; Γ ⊢ τ2 :: *@O.
 Proof.
   kind_inv_solver.
 Qed.
 
-Lemma kind_inv_let Σ Γ e τ κ :
-  Σ; Γ ⊢ let e in τ :: κ ->
+Lemma kind_inv_let Σ Φ Γ e τ κ :
+  Σ; Φ; Γ ⊢ let e in τ :: κ ->
   <{ *@O }> ⊑ κ /\
   exists τ' L,
-    Σ; Γ ⊢ e : τ' /\
-    (forall x, x ∉ L -> Σ; (<[x:=τ']> Γ) ⊢ τ^x :: *@O).
+    Σ; Φ; Γ ⊢ e : τ' /\
+    (forall x, x ∉ L -> Σ; Φ; (<[x:=τ']> Γ) ⊢ τ^x :: *@O).
 Proof.
   kind_inv_solver.
 Qed.
 
-Lemma kind_inv_case Σ Γ l e0 τ1 τ2 κ :
-  Σ; Γ ⊢ case{l} e0 of τ1 | τ2 :: κ ->
+Lemma kind_inv_case Σ Φ Γ l e0 τ1 τ2 κ :
+  Σ; Φ; Γ ⊢ case{l} e0 of τ1 | τ2 :: κ ->
   <{ *@O }> ⊑ κ /\
   l = ⊥ /\
   exists τ1' τ2' L1 L2,
-    Σ; Γ ⊢ e0 : τ1' + τ2' /\
-    (forall x, x ∉ L1 -> Σ; (<[x:=τ1']> Γ) ⊢ τ1^x :: *@O) /\
-    (forall x, x ∉ L2 -> Σ; (<[x:=τ2']> Γ) ⊢ τ2^x :: *@O).
+    Σ; Φ; Γ ⊢ e0 : τ1' + τ2' /\
+    (forall x, x ∉ L1 -> Σ; Φ; (<[x:=τ1']> Γ) ⊢ τ1^x :: *@O) /\
+    (forall x, x ∉ L2 -> Σ; Φ; (<[x:=τ2']> Γ) ⊢ τ2^x :: *@O).
 Proof.
   kind_inv_solver.
 Qed.
 
-Lemma kind_inv_mux Σ Γ e0 e1 e2 κ :
-  Σ; Γ ⊢ ~if e0 then e1 else e2 :: κ -> False.
+Lemma kind_inv_mux Σ Φ Γ e0 e1 e2 κ :
+  Σ; Φ; Γ ⊢ ~if e0 then e1 else e2 :: κ -> False.
 Proof.
   kind_inv_solver.
 Qed.
 
-Lemma kind_inv_sec Σ Γ e κ :
-  Σ; Γ ⊢ s𝔹 e :: κ -> False.
+Lemma kind_inv_sec Σ Φ Γ e κ :
+  Σ; Φ; Γ ⊢ s𝔹 e :: κ -> False.
 Proof.
   kind_inv_solver.
 Qed.
 
-Lemma kind_inv_pair Σ Γ e1 e2 κ :
-  Σ; Γ ⊢ (e1, e2) :: κ -> False.
+Lemma kind_inv_pair Σ Φ Γ e1 e2 κ :
+  Σ; Φ; Γ ⊢ (e1, e2) :: κ -> False.
 Proof.
   kind_inv_solver.
 Qed.
 
-Lemma kind_inv_proj Σ Γ b e κ :
-  Σ; Γ ⊢ π@b e :: κ -> False.
+Lemma kind_inv_proj Σ Φ Γ b e κ :
+  Σ; Φ; Γ ⊢ π@b e :: κ -> False.
 Proof.
   kind_inv_solver.
 Qed.
 
-Lemma kind_inv_inj Σ Γ l b τ e κ :
-  Σ; Γ ⊢ inj{l}@b<τ> e :: κ -> False.
+Lemma kind_inv_inj Σ Φ Γ l b τ e κ :
+  Σ; Φ; Γ ⊢ inj{l}@b<τ> e :: κ -> False.
 Proof.
   kind_inv_solver.
 Qed.
 
-Lemma kind_inv_ocase Σ Γ e0 e1 e2 κ :
-  Σ; Γ ⊢ ~case e0 of e1 | e2 :: κ -> False.
+Lemma kind_inv_ocase Σ Φ Γ e0 e1 e2 κ :
+  Σ; Φ; Γ ⊢ ~case e0 of e1 | e2 :: κ -> False.
 Proof.
   kind_inv_solver.
 Qed.
 
-Lemma kind_inv_fold Σ Γ X e κ :
-  Σ; Γ ⊢ fold<X> e :: κ -> False.
+Lemma kind_inv_fold Σ Φ Γ X e κ :
+  Σ; Φ; Γ ⊢ fold<X> e :: κ -> False.
 Proof.
   kind_inv_solver.
 Qed.
 
-Lemma kind_inv_unfold Σ Γ X e κ :
-  Σ; Γ ⊢ unfold<X> e :: κ -> False.
+Lemma kind_inv_unfold Σ Φ Γ X e κ :
+  Σ; Φ; Γ ⊢ unfold<X> e :: κ -> False.
 Proof.
   kind_inv_solver.
 Qed.
 
 Tactic Notation "apply_kind_inv" hyp(H) "by" tactic3(tac) :=
   lazymatch type of H with
-  | _; _ ⊢ Π:_, _ :: _ => tac kind_inv_pi
-  | _; _ ⊢ 𝔹 :: _ => tac kind_inv_bool
-  | _; _ ⊢ _ _ :: _ => tac kind_inv_app
-  | _; _ ⊢ let _ in _ :: _ => tac kind_inv_let
-  | _; _ ⊢ _ * _ :: _ => tac kind_inv_prod
-  | _; _ ⊢ _ + _ :: _ => tac kind_inv_sum
-  | _; _ ⊢ _ ~+ _ :: _ => tac kind_inv_osum
-  | _; _ ⊢ gvar _ :: _ => tac kind_inv_gvar
-  | _; _ ⊢ ~if _ then _ else _ :: _ => apply kind_inv_mux in H; elim H
-  | _; _ ⊢ if{_} _ then _ else _ :: _ => tac kind_inv_ite
-  | _; _ ⊢ ~case _ of _ | _ :: _ => apply kind_inv_ocase in H; elim H
-  | _; _ ⊢ case{_} _ of _ | _ :: _ => tac kind_inv_case
-  | _; _ ⊢ s𝔹 _ :: _ => apply kind_inv_sec in H; elim H
-  | _; _ ⊢ (_, _) :: _ => apply kind_inv_pair in H; elim H
-  | _; _ ⊢ π@_ _ :: _ => apply kind_inv_proj in H; elim H
-  | _; _ ⊢ inj{_}@_<_> _ :: _ => apply kind_inv_inj in H; elim H
-  | _; _ ⊢ fold<_> _ :: _ => apply kind_inv_fold in H; elim H
-  | _; _ ⊢ unfold<_> _ :: _ => apply kind_inv_unfold in H; elim H
+  | _; _; _ ⊢ Π:_, _ :: _ => tac kind_inv_pi
+  | _; _; _ ⊢ 𝔹 :: _ => tac kind_inv_bool
+  | _; _; _ ⊢ _ _ :: _ => tac kind_inv_app
+  | _; _; _ ⊢ let _ in _ :: _ => tac kind_inv_let
+  | _; _; _ ⊢ _ * _ :: _ => tac kind_inv_prod
+  | _; _; _ ⊢ _ + _ :: _ => tac kind_inv_sum
+  | _; _; _ ⊢ _ ~+ _ :: _ => tac kind_inv_osum
+  | _; _; _ ⊢ gvar _ :: _ => tac kind_inv_gvar
+  | _; _; _ ⊢ ~if _ then _ else _ :: _ => apply kind_inv_mux in H; elim H
+  | _; _; _ ⊢ if{_} _ then _ else _ :: _ => tac kind_inv_ite
+  | _; _; _ ⊢ ~case _ of _ | _ :: _ => apply kind_inv_ocase in H; elim H
+  | _; _; _ ⊢ case{_} _ of _ | _ :: _ => tac kind_inv_case
+  | _; _; _ ⊢ s𝔹 _ :: _ => apply kind_inv_sec in H; elim H
+  | _; _; _ ⊢ (_, _) :: _ => apply kind_inv_pair in H; elim H
+  | _; _; _ ⊢ π@_ _ :: _ => apply kind_inv_proj in H; elim H
+  | _; _; _ ⊢ inj{_}@_<_> _ :: _ => apply kind_inv_inj in H; elim H
+  | _; _; _ ⊢ fold<_> _ :: _ => apply kind_inv_fold in H; elim H
+  | _; _; _ ⊢ unfold<_> _ :: _ => apply kind_inv_unfold in H; elim H
   end.
 
 Tactic Notation "apply_kind_inv" hyp(H) :=
@@ -394,7 +396,7 @@ Tactic Notation "apply_kind_inv" "*" :=
 (** ** Type inversion *)
 Tactic Notation "type_inv_solver" "by" tactic3(tac) :=
   match goal with
-  | |- _; _ ⊢ ?e : _ -> _ => remember e
+  | |- _; _; _ ⊢ ?e : _ -> _ => remember e
   end;
   induction 1; subst; simp_hyps; simplify_eq;
   tac.
@@ -402,216 +404,216 @@ Tactic Notation "type_inv_solver" "by" tactic3(tac) :=
 Tactic Notation "type_inv_solver" :=
   type_inv_solver by (repeat esplit; eauto; equiv_naive_solver).
 
-Lemma type_inv_unit Σ Γ τ :
-  Σ; Γ ⊢ () : τ ->
-  Σ ⊢ τ ≡ 𝟙.
+Lemma type_inv_unit Σ Φ Γ τ :
+  Σ; Φ; Γ ⊢ () : τ ->
+  Σ; Φ ⊢ τ ≡ 𝟙.
 Proof.
   type_inv_solver.
 Qed.
 
-Lemma type_inv_lit Σ Γ b τ :
-  Σ; Γ ⊢ lit b : τ ->
-  Σ ⊢ τ ≡ 𝔹.
+Lemma type_inv_lit Σ Φ Γ b τ :
+  Σ; Φ; Γ ⊢ lit b : τ ->
+  Σ; Φ ⊢ τ ≡ 𝔹.
 Proof.
   type_inv_solver.
 Qed.
 
-Lemma type_inv_abs Σ Γ e τ2 τ :
-  Σ; Γ ⊢ \:τ2 => e : τ ->
+Lemma type_inv_abs Σ Φ Γ e τ2 τ :
+  Σ; Φ; Γ ⊢ \:τ2 => e : τ ->
   exists τ1 κ L,
-    Σ; Γ ⊢ τ2 :: κ /\
-    (forall x, x ∉ L -> Σ; (<[x:=τ2]> Γ) ⊢ e^x : τ1^x) /\
-    Σ ⊢ τ ≡ Π:τ2, τ1.
+    Σ; Φ; Γ ⊢ τ2 :: κ /\
+    (forall x, x ∉ L -> Σ; Φ; (<[x:=τ2]> Γ) ⊢ e^x : τ1^x) /\
+    Σ; Φ ⊢ τ ≡ Π:τ2, τ1.
 Proof.
   type_inv_solver.
 Qed.
 
-Lemma type_inv_gvar Σ Γ x τ :
-  Σ; Γ ⊢ gvar x : τ ->
+Lemma type_inv_gvar Σ Φ Γ x τ :
+  Σ; Φ; Γ ⊢ gvar x : τ ->
   exists τ' e,
     Σ !! x = Some (DFun τ' e) /\
-    Σ ⊢ τ ≡ τ'.
+    Σ; Φ ⊢ τ ≡ τ'.
 Proof.
   type_inv_solver.
 Qed.
 
-Lemma type_inv_pair Σ Γ e1 e2 τ :
-  Σ; Γ ⊢ (e1, e2) : τ ->
+Lemma type_inv_pair Σ Φ Γ e1 e2 τ :
+  Σ; Φ; Γ ⊢ (e1, e2) : τ ->
   exists τ1 τ2,
-    Σ; Γ ⊢ e1 : τ1 /\
-    Σ; Γ ⊢ e2 : τ2 /\
-    Σ ⊢ τ ≡ τ1 * τ2.
+    Σ; Φ; Γ ⊢ e1 : τ1 /\
+    Σ; Φ; Γ ⊢ e2 : τ2 /\
+    Σ; Φ ⊢ τ ≡ τ1 * τ2.
 Proof.
   type_inv_solver.
 Qed.
 
-Lemma type_inv_inj Σ Γ l b e τ' τ :
-  Σ; Γ ⊢ inj{l}@b<τ'> e : τ ->
+Lemma type_inv_inj Σ Φ Γ l b e τ' τ :
+  Σ; Φ; Γ ⊢ inj{l}@b<τ'> e : τ ->
   exists τ1 τ2,
     τ' = <{ τ1 +{l} τ2 }> /\
-    Σ; Γ ⊢ τ1 +{l} τ2 :: ite l *@O *@P /\
-    Σ; Γ ⊢ e : ite b τ1 τ2 /\
-    Σ ⊢ τ ≡ τ1 +{l} τ2.
+    Σ; Φ; Γ ⊢ τ1 +{l} τ2 :: ite l *@O *@P /\
+    Σ; Φ; Γ ⊢ e : ite b τ1 τ2 /\
+    Σ; Φ ⊢ τ ≡ τ1 +{l} τ2.
 Proof.
   type_inv_solver.
 Qed.
 
-Lemma type_inv_fold Σ Γ X e τ :
-  Σ; Γ ⊢ fold<X> e : τ ->
+Lemma type_inv_fold Σ Φ Γ X e τ :
+  Σ; Φ; Γ ⊢ fold<X> e : τ ->
   exists τ',
-    Σ; Γ ⊢ e : τ' /\
+    Σ; Φ; Γ ⊢ e : τ' /\
     Σ !! X = Some (DADT τ') /\
-    Σ ⊢ τ ≡ gvar X.
+    Σ; Φ ⊢ τ ≡ gvar X.
 Proof.
   type_inv_solver.
 Qed.
 
-Lemma type_inv_boxedlit Σ Γ b τ :
-  Σ; Γ ⊢ [b] : τ ->
-  Σ ⊢ τ ≡ ~𝔹.
+Lemma type_inv_boxedlit Σ Φ Γ b τ :
+  Σ; Φ; Γ ⊢ [b] : τ ->
+  Σ; Φ ⊢ τ ≡ ~𝔹.
 Proof.
   type_inv_solver.
 Qed.
 
-Lemma type_inv_boxedinj Σ Γ b v ω τ :
-  Σ; Γ ⊢ [inj@b<ω> v] : τ ->
+Lemma type_inv_boxedinj Σ Φ Γ b v ω τ :
+  Σ; Φ; Γ ⊢ [inj@b<ω> v] : τ ->
   exists ω1 ω2,
     ω = <{ ω1 ~+ ω2 }> /\
     oval <{ [inj@b<ω> v] }> ω /\
-    Σ ⊢ τ ≡ ω1 ~+ ω2.
+    Σ; Φ ⊢ τ ≡ ω1 ~+ ω2.
 Proof.
   type_inv_solver by hauto lq: on solve: equiv_naive_solver
                            ctrs: oval inv: oval.
 Qed.
 
-Lemma type_inv_case Σ Γ l e0 e1 e2 τ :
-  Σ; Γ ⊢ case{l} e0 of e1 | e2 : τ ->
+Lemma type_inv_case Σ Φ Γ l e0 e1 e2 τ :
+  Σ; Φ; Γ ⊢ case{l} e0 of e1 | e2 : τ ->
   exists τ1 τ2 τ' κ L1 L2,
-    Σ; Γ ⊢ τ' :: κ /\
-    Σ; Γ ⊢ e0 : τ1 +{l} τ2 /\
-    (forall x, x ∉ L1 -> Σ; (<[x:=τ1]> Γ) ⊢ e1^x : τ') /\
-    (forall x, x ∉ L2 -> Σ; (<[x:=τ2]> Γ) ⊢ e2^x : τ') /\
-    Σ ⊢ τ ≡ τ'.
+    Σ; Φ; Γ ⊢ τ' :: κ /\
+    Σ; Φ; Γ ⊢ e0 : τ1 +{l} τ2 /\
+    (forall x, x ∉ L1 -> Σ; Φ; (<[x:=τ1]> Γ) ⊢ e1^x : τ') /\
+    (forall x, x ∉ L2 -> Σ; Φ; (<[x:=τ2]> Γ) ⊢ e2^x : τ') /\
+    Σ; Φ ⊢ τ ≡ τ'.
 Proof.
   type_inv_solver.
 Qed.
 
-Lemma type_inv_ocase Σ Γ e0 e1 e2 τ :
-  Σ; Γ ⊢ ~case e0 of e1 | e2 : τ ->
+Lemma type_inv_ocase Σ Φ Γ e0 e1 e2 τ :
+  Σ; Φ; Γ ⊢ ~case e0 of e1 | e2 : τ ->
   exists τ1 τ2 τ' L1 L2,
-    Σ; Γ ⊢ τ' :: *@O /\
-    Σ; Γ ⊢ e0 : τ1 ~+ τ2 /\
-    (forall x, x ∉ L1 -> Σ; (<[x:=τ1]> Γ) ⊢ e1^x : τ') /\
-    (forall x, x ∉ L2 -> Σ; (<[x:=τ2]> Γ) ⊢ e2^x : τ') /\
-    Σ ⊢ τ ≡ τ'.
+    Σ; Φ; Γ ⊢ τ' :: *@O /\
+    Σ; Φ; Γ ⊢ e0 : τ1 ~+ τ2 /\
+    (forall x, x ∉ L1 -> Σ; Φ; (<[x:=τ1]> Γ) ⊢ e1^x : τ') /\
+    (forall x, x ∉ L2 -> Σ; Φ; (<[x:=τ2]> Γ) ⊢ e2^x : τ') /\
+    Σ; Φ ⊢ τ ≡ τ'.
 Proof.
   type_inv_solver.
 Qed.
 
-Lemma type_inv_prod Σ Γ τ1 τ2 τ :
-  Σ; Γ ⊢ τ1 * τ2 : τ -> False.
+Lemma type_inv_prod Σ Φ Γ τ1 τ2 τ :
+  Σ; Φ; Γ ⊢ τ1 * τ2 : τ -> False.
 Proof.
   type_inv_solver.
 Qed.
 
-Lemma type_inv_sum Σ Γ l τ1 τ2 τ :
-  Σ; Γ ⊢ τ1 +{l} τ2 : τ -> False.
+Lemma type_inv_sum Σ Φ Γ l τ1 τ2 τ :
+  Σ; Φ; Γ ⊢ τ1 +{l} τ2 : τ -> False.
 Proof.
   type_inv_solver.
 Qed.
 
-Lemma type_inv_app Σ Γ e1 e2 τ :
-  Σ; Γ ⊢ e1 e2 : τ ->
+Lemma type_inv_app Σ Φ Γ e1 e2 τ :
+  Σ; Φ; Γ ⊢ e1 e2 : τ ->
   exists τ1 τ2,
-    Σ; Γ ⊢ e1 : Π:τ2, τ1 /\
-    Σ; Γ ⊢ e2 : τ2 /\
-    Σ ⊢ τ ≡ τ1^e2.
+    Σ; Φ; Γ ⊢ e1 : Π:τ2, τ1 /\
+    Σ; Φ; Γ ⊢ e2 : τ2 /\
+    Σ; Φ ⊢ τ ≡ τ1^e2.
 Proof.
   type_inv_solver.
 Qed.
 
-Lemma type_inv_let Σ Γ e1 e2 τ :
-  Σ; Γ ⊢ let e1 in e2 : τ ->
+Lemma type_inv_let Σ Φ Γ e1 e2 τ :
+  Σ; Φ; Γ ⊢ let e1 in e2 : τ ->
   exists τ1 τ2 L,
-    Σ; Γ ⊢ e1 : τ1 /\
-    (forall x, x ∉ L -> Σ; (<[x:=τ1]> Γ) ⊢ e2^x : τ2^x) /\
-    Σ ⊢ τ ≡ τ2^e1.
+    Σ; Φ; Γ ⊢ e1 : τ1 /\
+    (forall x, x ∉ L -> Σ; Φ; (<[x:=τ1]> Γ) ⊢ e2^x : τ2^x) /\
+    Σ; Φ ⊢ τ ≡ τ2^e1.
 Proof.
   type_inv_solver.
 Qed.
 
-Lemma type_inv_sec Σ Γ e τ :
-  Σ; Γ ⊢ s𝔹 e : τ ->
-  Σ; Γ ⊢ e : 𝔹 /\
-  Σ ⊢ τ ≡ ~𝔹.
+Lemma type_inv_sec Σ Φ Γ e τ :
+  Σ; Φ; Γ ⊢ s𝔹 e : τ ->
+  Σ; Φ; Γ ⊢ e : 𝔹 /\
+  Σ; Φ ⊢ τ ≡ ~𝔹.
 Proof.
   type_inv_solver.
 Qed.
 
-Lemma type_inv_ite Σ Γ l e0 e1 e2 τ :
-  Σ; Γ ⊢ if{l} e0 then e1 else e2 : τ ->
+Lemma type_inv_ite Σ Φ Γ l e0 e1 e2 τ :
+  Σ; Φ; Γ ⊢ if{l} e0 then e1 else e2 : τ ->
   exists τ',
-    Σ; Γ ⊢ e0 : 𝔹{l} /\
-    Σ; Γ ⊢ e1 : τ' /\
-    Σ; Γ ⊢ e2 : τ' /\
-    Σ ⊢ τ ≡ τ'.
+    Σ; Φ; Γ ⊢ e0 : 𝔹{l} /\
+    Σ; Φ; Γ ⊢ e1 : τ' /\
+    Σ; Φ; Γ ⊢ e2 : τ' /\
+    Σ; Φ ⊢ τ ≡ τ'.
 Proof.
   type_inv_solver.
 Qed.
 
-Lemma type_inv_mux Σ Γ e0 e1 e2 τ :
-  Σ; Γ ⊢ ~if e0 then e1 else e2 : τ ->
+Lemma type_inv_mux Σ Φ Γ e0 e1 e2 τ :
+  Σ; Φ; Γ ⊢ ~if e0 then e1 else e2 : τ ->
   exists τ',
-    Σ; Γ ⊢ e0 : ~𝔹 /\
-    Σ; Γ ⊢ e1 : τ' /\
-    Σ; Γ ⊢ e2 : τ' /\
-    Σ; Γ ⊢ τ' :: *@O /\
-    Σ ⊢ τ ≡ τ'.
+    Σ; Φ; Γ ⊢ e0 : ~𝔹 /\
+    Σ; Φ; Γ ⊢ e1 : τ' /\
+    Σ; Φ; Γ ⊢ e2 : τ' /\
+    Σ; Φ; Γ ⊢ τ' :: *@O /\
+    Σ; Φ ⊢ τ ≡ τ'.
 Proof.
   type_inv_solver.
 Qed.
 
-Lemma type_inv_proj Σ Γ b e τ :
-  Σ; Γ ⊢ π@b e : τ ->
+Lemma type_inv_proj Σ Φ Γ b e τ :
+  Σ; Φ; Γ ⊢ π@b e : τ ->
   exists τ1 τ2,
-    Σ; Γ ⊢ e : τ1 * τ2 /\
-    Σ ⊢ τ ≡ ite b τ1 τ2.
+    Σ; Φ; Γ ⊢ e : τ1 * τ2 /\
+    Σ; Φ ⊢ τ ≡ ite b τ1 τ2.
 Proof.
   type_inv_solver.
 Qed.
 
-Lemma type_inv_unfold Σ Γ X e τ :
-  Σ; Γ ⊢ unfold<X> e : τ ->
+Lemma type_inv_unfold Σ Φ Γ X e τ :
+  Σ; Φ; Γ ⊢ unfold<X> e : τ ->
   exists τ',
     Σ !! X = Some (DADT τ') /\
-    Σ; Γ ⊢ e : gvar X /\
-    Σ ⊢ τ ≡ τ'.
+    Σ; Φ; Γ ⊢ e : gvar X /\
+    Σ; Φ ⊢ τ ≡ τ'.
 Proof.
   type_inv_solver.
 Qed.
 
 Tactic Notation "apply_type_inv" hyp(H) "by" tactic3(tac) :=
   lazymatch type of H with
-  | _; _ ⊢ () : _ => tac type_inv_unit
-  | _; _ ⊢ lit _ : _ => tac type_inv_lit
-  | _; _ ⊢ gvar _ : _ => tac type_inv_gvar
-  | _; _ ⊢ \:_ => _ : _ => tac type_inv_abs
-  | _; _ ⊢ _ _ : _ => tac type_inv_app
-  | _; _ ⊢ let _ in _ : _ => tac type_inv_let
-  | _; _ ⊢ (_, _) : _ => tac type_inv_pair
-  | _; _ ⊢ s𝔹 _ : _ => tac type_inv_sec
-  | _; _ ⊢ π@_ _ : _ => tac type_inv_proj
-  | _; _ ⊢ inj{_}@_<_> _ : _ => tac type_inv_inj
-  | _; _ ⊢ ~if _ then _ else _ : _ => tac type_inv_mux
-  | _; _ ⊢ if _ then _ else _ : _ => tac type_inv_ite
-  | _; _ ⊢ ~case _ of _ | _ : _ => tac type_inv_ocase
-  | _; _ ⊢ case{_} _ of _ | _ : _ => tac type_inv_case
-  | _; _ ⊢ fold<_> _ : _ => tac type_inv_fold
-  | _; _ ⊢ unfold<_> _ : _ => tac type_inv_unfold
-  | _; _ ⊢ [_] : _ => tac type_inv_boxedlit
-  | _; _ ⊢ [inj@_<_> _] : _ => tac type_inv_boxedinj
-  | _; _ ⊢ _ * _ : _ => apply type_inv_prod in H; elim H
-  | _; _ ⊢ _ +{_} _ : _ => apply type_inv_sum in H; elim H
+  | _; _; _ ⊢ () : _ => tac type_inv_unit
+  | _; _; _ ⊢ lit _ : _ => tac type_inv_lit
+  | _; _; _ ⊢ gvar _ : _ => tac type_inv_gvar
+  | _; _; _ ⊢ \:_ => _ : _ => tac type_inv_abs
+  | _; _; _ ⊢ _ _ : _ => tac type_inv_app
+  | _; _; _ ⊢ let _ in _ : _ => tac type_inv_let
+  | _; _; _ ⊢ (_, _) : _ => tac type_inv_pair
+  | _; _; _ ⊢ s𝔹 _ : _ => tac type_inv_sec
+  | _; _; _ ⊢ π@_ _ : _ => tac type_inv_proj
+  | _; _; _ ⊢ inj{_}@_<_> _ : _ => tac type_inv_inj
+  | _; _; _ ⊢ ~if _ then _ else _ : _ => tac type_inv_mux
+  | _; _; _ ⊢ if _ then _ else _ : _ => tac type_inv_ite
+  | _; _; _ ⊢ ~case _ of _ | _ : _ => tac type_inv_ocase
+  | _; _; _ ⊢ case{_} _ of _ | _ : _ => tac type_inv_case
+  | _; _; _ ⊢ fold<_> _ : _ => tac type_inv_fold
+  | _; _; _ ⊢ unfold<_> _ : _ => tac type_inv_unfold
+  | _; _; _ ⊢ [_] : _ => tac type_inv_boxedlit
+  | _; _; _ ⊢ [inj@_<_> _] : _ => tac type_inv_boxedinj
+  | _; _; _ ⊢ _ * _ : _ => apply type_inv_prod in H; elim H
+  | _; _; _ ⊢ _ +{_} _ : _ => apply type_inv_sum in H; elim H
   end.
 
 Tactic Notation "apply_type_inv" hyp(H) :=
@@ -650,11 +652,11 @@ Proof.
   qauto use: open_expr_wf_inv ctrs: expr_wf.
 Qed.
 
-Lemma typing_expr_wf Σ Γ e τ :
-  Σ; Γ ⊢ e : τ ->
+Lemma typing_expr_wf Σ Φ Γ e τ :
+  Σ; Φ; Γ ⊢ e : τ ->
   expr_wf e
-with kinding_expr_wf Σ Γ τ κ :
-  Σ; Γ ⊢ τ :: κ ->
+with kinding_expr_wf Σ Φ Γ τ κ :
+  Σ; Φ; Γ ⊢ τ :: κ ->
   expr_wf τ.
 Proof.
   all: destruct 1; eauto with expr_wf;
@@ -663,17 +665,17 @@ Qed.
 
 (** ** Properties of [otval] and [oval] *)
 
-Lemma otval_well_kinded ω Σ Γ :
+Lemma otval_well_kinded ω Σ Φ Γ :
   otval ω ->
-  Σ; Γ ⊢ ω :: *@O.
+  Σ; Φ; Γ ⊢ ω :: *@O.
 Proof.
   induction 1; hauto lq: on ctrs: kinding solve: lattice_naive_solver.
 Qed.
 
-Lemma otval_uniq Σ ω1 ω2 :
+Lemma otval_uniq Σ Φ ω1 ω2 :
   otval ω1 ->
   otval ω2 ->
-  Σ ⊢ ω1 ≡ ω2 ->
+  Σ; Φ ⊢ ω1 ≡ ω2 ->
   ω1 = ω2.
 Proof.
   intros H. revert ω2.
@@ -681,18 +683,18 @@ Proof.
     qauto l:on rew:off inv: otval.
 Qed.
 
-Lemma oval_elim v ω :
+Lemma oval_elim v ω:
   oval v ω ->
-  val v /\ otval ω /\ ∅; ∅ ⊢ v : ω.
+  val v /\ otval ω /\ forall Σ Φ Γ, Σ; Φ; Γ ⊢ v : ω.
 Proof.
   intros H. use H.
   induction H; hauto lq:on ctrs: val, otval, typing.
 Qed.
 
-Lemma oval_intro v ω Σ Γ :
+Lemma oval_intro v ω Σ Φ Γ :
   val v ->
   otval ω ->
-  Σ; Γ ⊢ v : ω ->
+  Σ; Φ; Γ ⊢ v : ω ->
   oval v ω.
 Proof.
   intros H. revert ω.
@@ -706,7 +708,7 @@ Proof.
 
   (* Case [inj@_<_> _] *)
   repeat match goal with
-         | H : _ ⊢ ?ω1 ≡ ?ω2 |- _ =>
+         | H : _; _ ⊢ ?ω1 ≡ ?ω2 |- _ =>
            apply otval_uniq in H; try qauto l: on inv: otval
          end.
 Qed.
@@ -721,8 +723,8 @@ Proof.
   sfirstorder use: (OVOSum true).
 Qed.
 
-Lemma any_kind_otval Σ Γ τ :
-  Σ; Γ ⊢ τ :: *@A ->
+Lemma any_kind_otval Σ Φ Γ τ :
+  Σ; Φ; Γ ⊢ τ :: *@A ->
   otval τ.
 Proof.
   remember <{ *@A }>.
