theories/lang_oadt/base.v
@@ -1,0 +1,20 @@
+From oadt Require Export prelude.
+
+Module Type OADTSig.
+
+  Context `(is_atom : Atom atom amap aset).
+
+  #[export]
+  Hint Resolve is_atom : typeclass_instances.
+
+  Parameter fset : forall A, EqDecision A -> Type.
+  Arguments fset _ {_}.
+  Context `(is_polyfinset : PolyFinSet fset).
+
+  #[export]
+  Hint Resolve is_polyfinset : typeclass_instances.
+
+End OADTSig.
+
+Declare Custom Entry oadt.
+Declare Custom Entry oadt_def.
