theories/lang_oadt/progress.v
@@ -1,12 +1,12 @@
-From oadt Require Import prelude.
+From oadt Require Import lang_oadt.base.
 From oadt Require Import lang_oadt.properties.
 
 (** * Progress *)
 (** The progress metatheorem. *)
 
-Module M (atom_sig : AtomSig).
+Module M (sig : OADTSig).
 
-Include properties.M atom_sig.
+Include properties.M sig.
 Import syntax_notations.
 Import semantics_notations.
 Import typing_notations.
@@ -25,57 +25,57 @@ Ltac canonical_form_solver :=
   apply_kind_inv;
   simpl_whnf_equiv.
 
-Lemma canonical_form_unit Σ Γ e :
+Lemma canonical_form_unit Σ Φ Γ e :
   val e ->
-  Σ; Γ ⊢ e : 𝟙 ->
+  Σ; Φ; Γ ⊢ e : 𝟙 ->
   e = <{ () }>.
 Proof.
   canonical_form_solver.
 Qed.
 
-Lemma canonical_form_abs Σ Γ e τ2 τ1 :
+Lemma canonical_form_abs Σ Φ Γ e τ2 τ1 :
   val e ->
-  Σ; Γ ⊢ e : Π:τ2, τ1 ->
+  Σ; Φ; Γ ⊢ e : Π:τ2, τ1 ->
   exists e' τ, e = <{ \:τ => e' }>.
 Proof.
   canonical_form_solver.
 Qed.
 
-Lemma canonical_form_bool Σ Γ e :
+Lemma canonical_form_bool Σ Φ Γ e :
   val e ->
-  Σ; Γ ⊢ e : 𝔹 ->
+  Σ; Φ; Γ ⊢ e : 𝔹 ->
   exists b, e = <{ b }>.
 Proof.
   canonical_form_solver.
 Qed.
 
-Lemma canonical_form_obool Σ Γ e :
+Lemma canonical_form_obool Σ Φ Γ e :
   val e ->
-  Σ; Γ ⊢ e : ~𝔹 ->
+  Σ; Φ; Γ ⊢ e : ~𝔹 ->
   exists b, e = <{ [b] }>.
 Proof.
   canonical_form_solver.
 Qed.
 
-Lemma canonical_form_prod Σ Γ e τ1 τ2 :
+Lemma canonical_form_prod Σ Φ Γ e τ1 τ2 :
   val e ->
-  Σ; Γ ⊢ e : τ1 * τ2 ->
+  Σ; Φ; Γ ⊢ e : τ1 * τ2 ->
   exists v1 v2, val v1 /\ val v2 /\ e = <{ (v1, v2) }>.
 Proof.
   canonical_form_solver.
 Qed.
 
-Lemma canonical_form_sum Σ Γ e τ1 τ2 :
+Lemma canonical_form_sum Σ Φ Γ e τ1 τ2 :
   val e ->
-  Σ; Γ ⊢ e : τ1 + τ2 ->
+  Σ; Φ; Γ ⊢ e : τ1 + τ2 ->
   exists b v τ, val v /\ e = <{ inj@b<τ> v }>.
 Proof.
   canonical_form_solver.
 Qed.
 
-Lemma canonical_form_osum Σ Γ e τ1 τ2 :
+Lemma canonical_form_osum Σ Φ Γ e τ1 τ2 :
   val e ->
-  Σ; Γ ⊢ e : τ1 ~+ τ2 ->
+  Σ; Φ; Γ ⊢ e : τ1 ~+ τ2 ->
   exists b v ω1 ω2, val v /\ otval ω1 /\ otval ω2 /\
                e = <{ [inj@b<ω1 ~+ ω2> v] }>.
 Proof.
@@ -87,9 +87,9 @@ Qed.
 
 (** Though it seems we should have a condition of [X] being an (public) ADT, this
 condition is not needed since it is implied by the typing judgment. *)
-Lemma canonical_form_fold Σ Γ e X :
+Lemma canonical_form_fold Σ Φ Γ e X :
   val e ->
-  Σ; Γ ⊢ e : gvar X ->
+  Σ; Φ; Γ ⊢ e : gvar X ->
   exists v X', val v /\ e = <{ fold<X'> v }>.
 Proof.
   inversion 1; inversion 1; intros; subst; eauto;
@@ -115,12 +115,12 @@ Ltac step_ectx_solver :=
 
 (** The combined progress theorems for expressions and types. *)
 Theorem progress_ Σ :
-  (forall Γ e τ,
-      Σ; Γ ⊢ e : τ ->
+  (forall Φ Γ e τ,
+      Σ; Φ; Γ ⊢ e : τ ->
       Γ = ∅ ->
       val e \/ exists e', Σ ⊨ e -->! e') /\
-  (forall Γ τ κ,
-     Σ; Γ ⊢ τ :: κ ->
+  (forall Φ Γ τ κ,
+     Σ; Φ; Γ ⊢ τ :: κ ->
      Γ = ∅ ->
      κ = <{ *@O }> ->
      otval τ \/ exists τ', Σ ⊨ τ -->! τ').
@@ -139,8 +139,6 @@ Proof.
           | match goal with
             | |- otval ?τ \/ _ => is_var τ
             end
-          (* Take care of the simple cases. *)
-          | goal_is (val <{ [inj@_<_> _] }> \/ _); sfirstorder use: oval_elim
           | qauto q: on rew: off
                   simp: simpl_map
                   ctrs: val, otval, step, ectx
@@ -168,12 +166,15 @@ Proof.
   (* [~case _ of _ | _] *)
   - right. intuition.
     (* Discriminee is value. *)
-    + select (_; _ ⊢ _ : _) (fun H => apply canonical_form_osum in H); eauto.
+    + select (_; _; _ ⊢ _ : _) (fun H => apply canonical_form_osum in H); eauto.
       simp_hyps.
       select! (otval _) (fun H => use (oval_inhabited _ H)).
       hauto ctrs: step.
     (* Discriminee can take a step. *)
     + hauto solve: step_ectx_solver ctrs: step.
+
+  (* [[inj@_<_> _]] *)
+  - sfirstorder use: oval_elim.
 
   (* [_ + _]. This case is impossible. *)
   - enough (<{ *@P }> ⊑ <{ *@O }>) by easy.
@@ -183,8 +184,8 @@ Proof.
   - select kind (fun κ => destruct κ); sintuition use: any_kind_otval.
 Qed.
 
-Theorem progress Σ τ e :
-  Σ; ∅ ⊢ e : τ ->
+Theorem progress Σ Φ τ e :
+  Σ; Φ; ∅ ⊢ e : τ ->
   val e \/ exists e', Σ ⊨ e -->! e'.
 Proof.
   hauto use: progress_.
